.

pure/Data.v
@@ -3,20 +3,14 @@ Require Import Coq.Bool.Bool.
 Require Import Coq.Classes.RelationClasses.
 Require Import Coq.Lists.List.
 Require Import Coq.micromega.Lia.
+Require Import Coq.Program.Basics.
+Require Import Coq.Program.Wf.
 Require Import DschingisKhan.pure.MyStructures.
 Require Import DschingisKhan.pure.MyUtilities.
 
 Module BinaryTrees.
 
   Import ListNotations EqFacts MyUtilities BasicSetoidTheory BasicPosetTheory.
-
-  Inductive bintree (Elem : Type) : Type :=
-  | BT_null : bintree Elem
-  | BT_node (lchild : bintree Elem) (element : Elem) (rchild : bintree Elem) : bintree Elem
-  .
-
-  Global Arguments BT_null {Elem}.
-  Global Arguments BT_node {Elem}.
 
   Section INDICES_OF_BINARY_TREES.
 
@@ -25,11 +19,31 @@ Module BinaryTrees.
   | Dir_right : dir_t
   .
 
-  Definition encode (ds : list dir_t) : nat :=
-    fold_left (fun code : nat => dir_t_rect (fun _ => nat) (2 * code + 1) (2 * code + 2)) ds 0
+  Definition encode : list dir_t -> nat :=
+    fun ds : list dir_t =>
+    fold_left (fun code : nat => @dir_t_rect (fun _ : dir_t => nat) (2 * code + 1) (2 * code + 2)) ds 0
   .
 
-  Lemma decode (code : nat) :
+  Lemma encode_inj :
+    forall ds1 : list dir_t,
+    forall ds2 : list dir_t,
+    encode ds1 = encode ds2 ->
+    ds1 = ds2.
+  Proof with lia || eauto.
+    unfold encode; intros ds1 ds2. do 2 rewrite <- fold_left_rev_right.
+    intros H_eq; apply list_rev_inj; revert H_eq.
+    generalize (rev ds2) as xs2. generalize (rev ds1) as xs1. clear ds1 ds2.
+    set (myF := fold_right (fun y : dir_t => fun x : nat => @dir_t_rect (fun _ : dir_t => nat) (2 * x + 1) (2 * x + 2) y) 0).
+    induction xs1 as [ | x1 xs1 IH]; destruct xs2 as [ | x2 xs2]; simpl...
+    - destruct x2; simpl dir_t_rect...
+    - destruct x1; simpl dir_t_rect...
+    - destruct x1; destruct x2; simpl dir_t_rect...
+      all: intros H_eq; assert (claim1 : myF xs1 = myF xs2)...
+      all: apply eq_congruence...
+  Qed.
+
+  Lemma decodable :
+    forall code : nat,
     {ds : list dir_t | encode ds = code}.
   Proof with lia || eauto.
     induction code as [[ | n'] IH] using Wf_nat.lt_wf_rect1.
@@ -53,44 +67,189 @@ Module BinaryTrees.
       + pose (Nat.mod_bound_pos code 2)...
   Defined.
 
+  Definition decode : nat -> list dir_t :=
+    fun code : nat =>
+    proj1_sig (decodable code)
+  .
+
 (*
-  Compute (proj1_sig (decode 14)).
+  Compute (decode 14).
   (* = [Dir_right; Dir_right; Dir_right] *)
-  Compute (proj1_sig (decode 15)).
+  Compute (decode 15).
   (* = [Dir_left; Dir_left; Dir_left; Dir_left] *)
-  Compute (proj1_sig (decode 16)).
+  Compute (decode 16).
   (* = [Dir_left; Dir_left; Dir_left; Dir_right] *)
 *)
 
-  Lemma encode_inj :
-    forall ds1 : list dir_t,
-    forall ds2 : list dir_t,
-    encode ds1 = encode ds2 ->
-    ds1 = ds2.
-  Proof with lia || eauto.
-    unfold encode; intros ds1 ds2. do 2 rewrite <- fold_left_rev_right.
-    intros H_eq; apply list_rev_inj; revert H_eq.
-    generalize (rev ds2) as xs2. generalize (rev ds1) as xs1. clear ds1 ds2.
-    set (myF := fold_right (fun y : dir_t => fun x : nat => dir_t_rect (fun _ : dir_t => nat) (2 * x + 1) (2 * x + 2) y) 0).
-    induction xs1 as [ | x1 xs1 IH]; destruct xs2 as [ | x2 xs2]; simpl...
-    - destruct x2; simpl dir_t_rect...
-    - destruct x1; simpl dir_t_rect...
-    - destruct x1; destruct x2; simpl dir_t_rect...
-      all: intros H_eq; assert (claim1 : myF xs1 = myF xs2)...
-      all: apply f_equal...
+  Lemma encode_decode :
+    forall code : nat,
+    encode (decode code) = code.
+  Proof.
+    exact (fun code : nat => proj2_sig (decodable code)).
+  Qed.
+
+  Global Opaque decode.
+
+  Lemma decode_encode :
+    forall ds : list dir_t,
+    decode (encode ds) = ds.
+  Proof.
+    intro ds.
+    apply encode_inj.
+    now rewrite encode_decode with (code := encode ds).
   Qed.
 
   End INDICES_OF_BINARY_TREES.
 
-  Fixpoint option_subtree {A : Type} (ds : list dir_t) (t : bintree A) {struct ds} : option (bintree A) :=
+  Inductive bintree (Elem : Type) : Type :=
+  | BT_null : bintree Elem
+  | BT_node (lchild : bintree Elem) (element : Elem) (rchild : bintree Elem) : bintree Elem
+  .
+
+  Global Arguments BT_null {Elem}.
+  Global Arguments BT_node {Elem}.
+
+  Definition option_elem {Elem : Type} (t : bintree Elem) : option Elem :=
+    match t with
+    | BT_null => None
+    | BT_node t_l t_e t_r => Some t_e
+    end
+  .
+
+  Definition option_children_pair {Elem : Type} (t : bintree Elem) : option (bintree Elem * bintree Elem) :=
+    match t with
+    | BT_null => None
+    | BT_node t_l t_e t_r => Some (t_l, t_r)
+    end
+  .
+
+  Definition option_subtree {Elem : Type} : list dir_t -> bintree Elem -> option (bintree Elem) :=
+    fix option_subtree_fix (ds : list dir_t) (t : bintree Elem) {struct ds} : option (bintree Elem) :=
     match ds with
     | [] => Some t
-    | d :: ds' =>
+    | d :: ds =>
       match t with
       | BT_null => None
-      | BT_node l e r => option_subtree ds' (dir_t_rect (fun _ => bintree A) l r d)
+      | BT_node t_l t_e t_r => option_subtree_fix ds (@dir_t_rect (fun _ : dir_t => bintree Elem) t_l t_r d)
       end
     end
   .
+
+  Section BINARY_TREE_TO_LIST.
+
+  Definition option2list {A : Type} : option A -> list A :=
+    @option_rect A (fun _ => list A) (fun x : A => [x]) []
+  .
+
+  Definition pair2list {A : Type} : A * A -> list A :=
+    fun pr : A * A =>
+    [fst pr; snd pr]
+  .
+
+  Context {Elem : Type}.
+
+  Let cnt : bintree Elem -> nat :=
+    fix cnt_fix (t : bintree Elem) {struct t} : nat :=
+    match t with
+    | BT_null => 1
+    | BT_node t_l t_e t_r => 1 + cnt_fix t_l + cnt_fix t_r
+    end
+  .
+
+  Program Fixpoint toList_step (ts : list (bintree Elem)) {measure (list_sum (map cnt ts))} : list Elem :=
+    match ts with
+    | [] => []
+    | BT_null :: ts_tail => toList_step ts_tail
+    | BT_node t_l t_e t_r :: ts_tail => t_e :: toList_step ((ts_tail ++ [t_l]) ++ [t_r])
+    end.
+  Next Obligation.
+    unfold Peano.lt.
+    do 2 rewrite map_last. do 2 rewrite list_sum_app; cbn.
+    do 2 rewrite Nat.add_0_r. rewrite <- Nat.add_assoc at 1.
+    rewrite Nat.add_comm; constructor.
+  Defined.
+
+  Lemma toList_step_unfold :
+    forall ts : list (bintree Elem),
+    toList_step ts =
+    match ts with
+    | [] => []
+    | BT_null :: ts_tail => toList_step ts_tail
+    | BT_node t_l t_e t_r :: ts_tail => t_e :: toList_step (ts_tail ++ [t_l; t_r])
+    end.
+  Proof with eauto.
+    intros ts. unfold toList_step at 1; rewrite fix_sub_eq.
+    - destruct ts as [ | [ | t_l t_e t_r] ts_tail]...
+      simpl; apply f_equal.
+      replace ((ts_tail ++ [t_l]) ++ [t_r]) with (ts_tail ++ [t_l; t_r]) at 1...
+      rewrite <- app_assoc...
+    - intros [ | [ | ? ? ?] ?] ? ? ?...
+      apply f_equal...
+  Qed.
+
+  Global Opaque toList_step.
+
+  Local Open Scope program_scope.
+
+  Definition extract_elements : list (bintree Elem) -> list Elem :=
+    flat_map (option2list ∘ option_elem)
+  .
+
+  Definition extract_children : list (bintree Elem) -> list (bintree Elem) :=
+    flat_map (@concat (bintree Elem) ∘ option2list ∘ option_map pair2list ∘ option_children_pair)
+  .
+
+  Lemma extract_elements_unfold :
+    forall ts : list (bintree Elem),
+    extract_elements ts =
+    match ts with
+    | [] => []
+    | BT_null :: ts_tail => extract_elements ts_tail
+    | BT_node t_l t_e t_r :: ts_tail => t_e :: extract_elements ts_tail
+    end.
+  Proof.
+    destruct ts as [ | [ | ? ? ?] ?]; reflexivity.
+  Qed.
+
+  Lemma extract_children_unfold :
+    forall ts : list (bintree Elem),
+    extract_children ts =
+    match ts with
+    | [] => []
+    | BT_null :: ts_tail => extract_children ts_tail
+    | BT_node t_l t_e t_r :: ts_tail => [t_l; t_r] ++ extract_children ts_tail
+    end.
+  Proof.
+    destruct ts as [ | [ | ? ? ?] ?]; reflexivity.
+  Qed.
+
+  Lemma toList_step_app :
+    forall prevs : list (bintree Elem),
+    forall nexts : list (bintree Elem),
+    toList_step (prevs ++ nexts) =
+    extract_elements prevs ++ toList_step (nexts ++ extract_children prevs).
+  Proof with eauto with *.
+    induction prevs as [ | [ | t_l t_e t_r] prevs IH]; simpl.
+    all: intros nexts; autorewrite with list...
+    { rewrite toList_step_unfold... }
+    { rewrite toList_step_unfold, <- app_assoc, IH, <- app_assoc... }
+  Qed.
+
+  Theorem toList_step_spec :
+    forall ts : list (bintree Elem),
+    toList_step ts =
+    extract_elements ts ++ toList_step (extract_children ts).
+  Proof.
+    intros ts.
+    replace (ts) with (ts ++ []) at 1.
+    - exact (toList_step_app ts []).
+    - apply app_nil_r.
+  Qed.
+
+  Definition toList (root : bintree Elem) : list Elem :=
+    toList_step [root]
+  .
+
+  End BINARY_TREE_TO_LIST.
 
 End BinaryTrees.
